x86/Conventions1C.v
@@ -28,3 +28,33 @@ Proof.
   rewrite loc_arguments_length_aux. ss.
 Qed.
 
+Local Opaque Z.add Z.mul Z.sub Z.div.
+Local Opaque list_nth_z.
+
+Let size_arguments_loc_arguments_aux: forall
+    tys
+    ofs
+    x y z
+    (IN: z <= ofs < size_arguments_64 tys x y z)
+  ,
+    exists base ty, <<IN: In (S Outgoing base ty) (regs_of_rpairs (loc_arguments_64 tys x y z))>>
+.
+Proof.
+  i. ginduction tys; ii; ss.
+  { xomega. }
+  destruct a; ss; des_ifs; ss; try (by esplits; eauto);
+    try (exploit IHtys; eauto; []; i; des; []); try (by esplits; eauto).
+Qed.
+
+Lemma size_arguments_loc_arguments
+      sg ofs
+      (IN: 0 <= ofs < size_arguments sg)
+  :
+    exists ofs ty, <<IN: In (S Outgoing ofs ty) (regs_of_rpairs (loc_arguments sg))>>
+.
+Proof.
+  destruct sg; ss.
+  unfold size_arguments, loc_arguments in *. ss. des_ifs. clear_tac.
+  eapply size_arguments_loc_arguments_aux; eauto.
+Qed.
+
